@prefix hsml: <https://www.spatialwebfoundation.org/ns/hsml#> .
@prefix owl: <http://www.w3.org/2002/07/owl#> .
@prefix rdfs: <http://www.w3.org/2000/01/rdf-schema#> .

hsml:authorizedAgent a owl:ObjectProperty ;
    rdfs:label "authorized agent" ;
    rdfs:comment "Links a Channel to the Agent(s) permitted to access it; only those Agents holding the necessary credentials or roles may use this Channel." ;
    rdfs:range hsml:Agent .

hsml:isChannelFor a owl:ObjectProperty ;
    rdfs:label "is channel for" ;
    rdfs:comment "Links a Channel to the Activity (or Activities) whose messages it carries." ;
    rdfs:range hsml:Activity .

hsml:hasSubChannel a owl:ObjectProperty ;
    rdfs:label "has subchannel" ;
    rdfs:comment "Indicates that this Channel has the given Channel as a sub-channel." ;
    rdfs:range hsml:Channel ;
    owl:inverseOf hsml:isSubChannelOf .

hsml:isSubChannelOf a owl:ObjectProperty ;
    rdfs:label "subChannelOf" ;
    rdfs:comment "Indicates that this Channel is a sub-channel of another Channel" ;
    rdfs:range hsml:Channel ;
    owl:inverseOf hsml:hasSubChannel .

hsml:Channel a owl:Class ;
    rdfs:label "Channel" ;
    rdfs:comment "A CHANNEL is a Spatial Web ENTITY grouping a stream of HSML elements related to a specific context or communication without warranting a domain hierarchy. " ;
    rdfs:subClassOf hsml:Entity .

