@prefix hsml: <https://www.spatialwebfoundation.org/ns/hsml#> .
@prefix owl: <http://www.w3.org/2002/07/owl#> .
@prefix rdfs: <http://www.w3.org/2000/01/rdf-schema#> .

hsml:Concept a owl:Class ;
    rdfs:label "Concept" ;
    rdfs:comment "A domain that contains intangible concepts and abstract ideas thatmy not have physical presence, but hold significance for a community of users. " ;
    rdfs:subClassOf hsml:Domain .

hsml:SpatialFeature a owl:Class ;
    rdfs:label "Spatial Feature" ;
    rdfs:comment "A domain that refers to the features of worlds including the earth, the moon, planets and virtual worlds. Domains of this type may have several geometric representations." ;
    rdfs:subClassOf hsml:Domain .

hsml:Thing a owl:Class ;
    rdfs:label "Thing" ;
    rdfs:comment "A THING is a passive DOMAIN representing bounded items without agency that can be acted upon or manipulated by AGENTs." ;
    rdfs:subClassOf hsml:Domain .

hsml:domainAuthority a owl:ObjectProperty ;
    rdfs:label "domain authority" ;
    rdfs:comment "Specifies the Domain Authority responsible for governance, policies, and contracts within this Domain" ;
    rdfs:range hsml:Agent .

hsml:hasActivitySchema a owl:ObjectProperty ;
    rdfs:label "has activity schema" ;
    rdfs:comment "Specifies the activity schemas that can be performed in/on/by/with the domain" ;
    rdfs:range hsml:ActivitySchema .

hsml:hasSubDomain a owl:ObjectProperty ;
    rdfs:label "hasSubDomain" ;
    rdfs:comment "Links a parent Domain to one or more child Domains that it contains or specializes, capturing nested or hierarchical relationships among Domains." ;
    rdfs:range hsml:Domain ;
    owl:inverseOf hsml:subDomainOf .

hsml:subDomainOf a owl:ObjectProperty ;
    rdfs:label "subDomainOf" ;
    rdfs:comment "Links a domain to its immediate parent domain in a hierarchical domain structure. Inverse of hsml:hasSubDomain" ;
    rdfs:range hsml:Domain ;
    owl:inverseOf hsml:hasSubDomain .

hsml:Domain a owl:Class ;
    rdfs:label "Domain" ;
    rdfs:comment "A DOMAIN is a Spatial Web ENTITY with identity through time endowed with rights and credentials." ;
    rdfs:subClassOf hsml:Entity .

