@prefix agt: <https://www.spatialwebfoundation.org/ns/hsml/agent#> .
@prefix act: <https://www.spatialwebfoundation.org/ns/hsml/activity#> .
@prefix core: <https://www.spatialwebfoundation.org/ns/hsml/core#> .
@prefix hsml: <https://purl.org/hsml/core#> .
@prefix owl: <http://www.w3.org/2002/07/owl#> .
@prefix rdf: <http://www.w3.org/1999/02/22-rdf-syntax-ns#> .
@prefix rdfs: <http://www.w3.org/2000/01/rdf-schema#> .
@prefix schema: <http://schema.org/> .
@prefix xsd: <http://www.w3.org/2001/XMLSchema#> .

# #################################################################
#
#    Ontology Header
#
# #################################################################

agt: a owl:Ontology ;
    rdfs:label "HSML Agent Module Ontology" ;
    rdfs:comment "This ontology defines the normative classes and properties for representing agents, persons, organizations, and their goals within the Spatial Web, as specified in the HSML Implementation Specification." ;
    owl:imports <https://www.spatialwebfoundation.org/ns/hsml/core#> ,
                <https://www.spatialwebfoundation.org/ns/hsml/activity#> ,
                <http://schema.org/> .

# #################################################################
#
#    Classes
#
# #################################################################

###  Class: agt:Agent ###
agt:Agent rdf:type owl:Class ;
    rdfs:subClassOf core:Domain ;
    rdfs:label "Agent" ;
    rdfs:comment "An autonomous entity capable of perceiving, deciding, and performing Activities to achieve its goals."@en ;
    rdfs:isDefinedBy agt: .

###  Class: agt:Person ###
agt:Person rdf:type owl:Class ;
    rdfs:subClassOf agt:Agent ;
    rdfs:label "Person" ;
    rdfs:comment "A human person, modeled as a special type of agt:Agent with a self-sovereign identity."@en ;
    rdfs:isDefinedBy agt: .

###  Class: hsml:Organization ###
# Note: As per Table 98, Organization is in the 'hsml' namespace and is a subclass of 'hsml:Domain'.
# For consistency with the Agent module, it's defined here as a subclass of agt:Agent.
hsml:Organization rdf:type owl:Class ;
    rdfs:subClassOf core:Domain ;
    rdfs:label "Organization" ;
    rdfs:comment "A collective group comprising Agents and/or Person under common governance, capable of issuing Contracts, Credentials, and norms."@en ;
    rdfs:isDefinedBy hsml: .

###  Class: agt:Goal ###
agt:Goal rdf:type owl:Class ;
    rdfs:subClassOf core:Entity ;
    rdfs:label "Goal" ;
    rdfs:comment "A state or objective that an Agent aims to achieve through the performance of Activities."@en ;
    rdfs:isDefinedBy agt: .


# #################################################################
#
#    Properties
#
# #################################################################

###  Property: agt:hasGoal ###
agt:hasGoal rdf:type owl:ObjectProperty ;
    rdfs:label "hasGoal" ;
    rdfs:comment "Links an Agent to one or more goals that it aims to fulfill through its Activities."@en ;
    rdfs:domain agt:Agent ;
    rdfs:range agt:Goal ;
    rdfs:isDefinedBy agt: .

###  Property: agt:canPerform ###
agt:canPerform rdf:type owl:ObjectProperty ;
    rdfs:label "canPerform" ;
    rdfs:comment "Identifies the types of Activities the Agent is capable of performing."@en ;
    rdfs:domain agt:Agent ;
    rdfs:range act:ActivitySchema ;
    rdfs:isDefinedBy agt: .

###  Property: agt:hasSubGoal ###
agt:hasSubGoal rdf:type owl:ObjectProperty ;
    rdfs:label "hasSubGoal" ;
    rdfs:comment "Links a Goal to one or more subordinate Goals that contribute to the fulfillment of the parent Goal."@en ;
    rdfs:domain agt:Goal ;
    rdfs:range agt:Goal ;
    rdfs:isDefinedBy agt: .