@prefix hsml: <https://www.spatialwebfoundation.org/ns/hsml#> .
@prefix owl: <http://www.w3.org/2002/07/owl#> .
@prefix rdfs: <http://www.w3.org/2000/01/rdf-schema#> .

hsml:Organization a owl:Class ;
    rdfs:label "Organization" ;
    rdfs:comment "An ORGANIZATION is an AGENT representing a collective domain with decisionâ€‘making capabilities and governance structures." ;
    rdfs:subClassOf hsml:Agent .

hsml:Person a owl:Class ;
    rdfs:label "Person" ;
    rdfs:comment "A PERSON is an AGENT representing a human individual with persistent identity and agency." ;
    rdfs:subClassOf hsml:Agent .

hsml:embodiedIn a owl:ObjectProperty ;
    rdfs:label "embodied in" ;
    rdfs:comment "Links an Agent to the physical Thing it inhabits" ;
    rdfs:range hsml:Thing .

hsml:hasCapability a owl:ObjectProperty ;
    rdfs:label "has capability" ;
    rdfs:comment "Links an Agent to it capability (sensing,and perceiving, activity schemas, learning mechanisms, autonomous decision-making, physical and digital actuations)" ;
    rdfs:range hsml:Capability .

hsml:hasGoal a owl:ObjectProperty ;
    rdfs:label "has goal" ;
    rdfs:comment "A goal or desired outcome that this agent aims to accomplish" ;
    rdfs:range hsml:Goal .

hsml:performsActivity a owl:ObjectProperty ;
    rdfs:label "performs activity" ;
    rdfs:comment "An activity that this agent has performed or is performing." ;
    rdfs:range hsml:Activity .

hsml:situation a owl:ObjectProperty ;
    rdfs:label "situation" ;
    rdfs:comment "A situation relationship is an entity comprised of all DOMAINS that can be perceived and reasoned about by an AGENT" ;
    rdfs:range hsml:Entity .

hsml:usesTool a owl:ObjectProperty ;
    rdfs:label "uses tool" ;
    rdfs:comment "Indicates that an Agent employs a Tool in pursuit of its goals" ;
    rdfs:range hsml:Tool .

hsml:Agent a owl:Class ;
    rdfs:label "Agent" ;
    rdfs:comment "An AGENT is an ENTITY that senses and responds to its environment, maintains a model of its environment, and performs ACTIVITIES to achieve its goals." ;
    rdfs:subClassOf hsml:Domain .

